iso_dh/initiator.v
@@ -43,25 +43,23 @@ Definition initiator : val := λ: "c" "skI" "vkR",
 Ltac protocol_failure :=
   by intros; wp_pures; iApply ("Hpost" $! None); iFrame.
 
-Lemma wp_initiator c kI kR dq n :
+Lemma wp_initiator c kI kR :
   channel c -∗
   cryptis_ctx -∗
   iso_dh_ctx N -∗
   public (TKey Open kI) -∗
   public (TKey Open kR) -∗
-  {{{ ●Ph{dq} n }}}
+  {{{ True }}}
     initiator c kI (TKey Open kR)
   {{{ okS, RET (repr okS);
-      ●Ph{dq} n ∗
       if okS is Some kS then ∃ si,
         ⌜si_init si = kI⌝ ∗
         ⌜si_resp si = kR⌝ ∗
         ⌜si_key si = kS⌝ ∗
-        ⌜si_time si = n⌝ ∗
         minted kS ∗
-        □ (∀ kt, public (TKey kt kS) ↔ ▷ session_fail si) ∗
-        term_token (si_init_share si) ⊤ ∗
-        (session_fail si ∨ session si)
+        □ (∀ kt, public (TKey kt kS) ↔ ◇ public kS) ∗
+        (public (TKey Seal kR) ∨ □ (◇ public kS ↔ ▷ False)) ∗
+        term_token (si_init_share si) ⊤
       else True
  }}}.
 Proof.
@@ -69,24 +67,18 @@ rewrite /initiator.
 set vkI := TKey Open kI.
 set vkR := TKey Open kR.
 iIntros "#chan_c #ctx #(? & ?) #p_kI #p_kR %Ψ !> phase Hpost".
-iMod (minted_at_list with "[] phase") as "[phase list]" => //; eauto.
-wp_pures.
-iDestruct "list" as "(%M & #m_M & #minted_at_M)".
-wp_apply wp_vkey. wp_pures. rewrite -/vkI.
-wp_bind (mknonce _).
-iApply (wp_mknonce_freshN M
-          (λ _, public_at n (TKey Seal kI) ∨
-                public_at n (TKey Seal kR))%I
-          iso_dh_pred
-          (λ a, {[TExp (TInt 0) a]})) => //.
-- iIntros "% ?". rewrite big_sepS_forall. by iApply "m_M".
+wp_pures. wp_apply wp_vkey. wp_pures. rewrite -/vkI.
+wp_apply (wp_mknonce_freshN ∅
+            (λ _, False%I)
+            iso_dh_pred
+            (λ a, {[TExp (TInt 0) a]})) => //.
+- iIntros "% ?". by rewrite elem_of_empty.
 - iIntros "%a". rewrite big_sepS_singleton minted_TExp minted_TInt /=.
   iIntros "!>"; iSplit; eauto.
   by iIntros "(_ & ?)".
 iIntros "%a %fresh %nonce #m_a #s_a #a_pred token".
 set ga := TExp (TInt 0) a.
 rewrite big_sepS_singleton.
-iPoseProof (phase_auth_frag with "phase") as "#phaseI".
 wp_pures. wp_apply wp_mkkeyshare => //. rewrite -/ga.
 iIntros "_". wp_pures. wp_list. wp_term_of_list.
 wp_pure _ credit:"H1".
@@ -97,11 +89,10 @@ iAssert (public ga) as "p_ga".
   iRight. do 2![iSplit => //].
   iApply "a_pred". iModIntro. iModIntro.
   by rewrite /iso_dh_pred exps_TExpN. }
-wp_bind (send _ _). iApply wp_send => //.
-{ rewrite public_of_list /=. iModIntro.
-  do 2?[iSplit => //]. }
+wp_apply wp_send => //.
+{ rewrite public_of_list /=. do 2?[iSplit => //]. }
 wp_pure _ credit:"H3".
-wp_pures. wp_bind (recv _). iApply wp_recv => //.
+wp_pures. wp_apply wp_recv => //.
 iIntros "%m2 #p_m2".
 wp_verify m2; last by protocol_failure.
 wp_pures. wp_list_of_term m2; last by protocol_failure.
@@ -125,93 +116,43 @@ set gab := TExp gb a.
 set seed := Spec.of_list [vkI; vkR; ga; gb; gab].
 set secret := Spec.derive_key seed.
 wp_pures. wp_list. wp_term_of_list. wp_apply wp_sign. wp_pures.
-iAssert ( |={⊤}=>
-    ●Ph{dq} n ∗
-    (public_at n (TKey Seal kR) ∨
-    ∃ b,
-     ⌜gb = TExp (TInt 0) b⌝ ∗
-     □ (public b ↔ ▷ □ (public_at n (TKey Seal kI) ∨
-                        public_at n (TKey Seal kR))) ∗
-     term_meta secret (nroot.@"info") n))%I
-  with "[phase H3]"
-  as "{p_m2} > (phase & p_m2)".
+iAssert (|={⊤}=> public (TKey Seal kR) ∨ □ (◇ public secret ↔ ▷ False))%I
+  with "[H3]"
+  as "{p_m2} > #p_m2".
 { iPoseProof (public_TSealE with "p_m2 [//]") as "{p_m2} p_m2".
-  iDestruct "p_m2" as "[[comp _]  | (#i_m2 & _ & _)]".
-  { by iMod (public_atI with "[ctx] [H3] [phase] [comp]")
-      as "[phase #comp']" => //; try solve_ndisj. }
+  iDestruct "p_m2" as "[[comp _]  | (#i_m2 & _ & _)]"; first by eauto.
   iMod (lc_fupd_elim_later_pers with "H3 i_m2") as "{i_m2} #i_m2".
-  iDestruct "i_m2"
-    as "(%ga' & %b & %kI' & %n' & %e_m2 & m_ga & s_b & pred_b & meta)".
-  case/Spec.of_list_inj: e_m2 => <- -> <- {ga' gb kI'} in gab seed secret *.
-  case: (decide (n' < n)) => [contra|?].
-  { iPoseProof ("minted_at_M" with "[//] m_ga") as "%ga_M".
-    move/(_ _ ga_M)/subtermsP: fresh.
-    rewrite subterms_TExpN // !elem_of_union => fresh.
-    case: fresh.
-    right. right. left. apply/subtermsP. apply/STRefl. }
-  iPoseProof (minted_at_phase_frag with "m_ga") as "#phaseR".
-  iPoseProof (phase_auth_frag_agree with "phase phaseR") as "%".
-  have ? : n' = n by lia. subst n'.
-  rewrite /secret /seed /gab !TExp_TExpN TExpC2. iFrame.
-  iModIntro. iRight. iExists b. iFrame.
-  iSplit => //.
-  iSplit => //.
-  iModIntro. iSplit.
-  - iIntros "#p_b".
-    iSpecialize ("s_b" with "p_b").
-    do 2!iModIntro.
-    iDestruct "s_b" as "#[(% & %e & ?)|?]"; last by eauto.
-    case: e => <-; by eauto.
-  - iIntros "#fail"; iApply "s_b".
-    iModIntro.
-    iDestruct "fail" as "[fail|fail]"; eauto. }
+  iDestruct "i_m2" as "(%ga' & %b & %kI' & %e_m2 & s_b & pred_b)".
+  case/Spec.of_list_inj: e_m2 => _ -> _ {ga' gb kI'} in gab seed secret *.
+  rewrite !TExp_TExpN TExpC2 in gab seed secret *.
+  iIntros "!>". iRight. iIntros "!>".
+  rewrite public_derive_key public_of_list /=.
+  iApply (bi.iff_trans _ (◇ public gab)).
+  iSplit; last by iApply public_dh_secret.
+  iSplit; last by iIntros "#?"; do !iSplit.
+  by iIntros ">(_ & _ & _ & _ & ? & _)". }
 set m3 := Spec.enc _ _ _.
 iAssert (public m3) as "#p_m3".
 { iApply (public_TSealIS with "[] [//] [#]") => //.
   - by rewrite !public_minted !minted_TKey.
-  - iExists a, gb, kR, n. do 3![iSplitR => //].
-    iDestruct "p_m2" as "[#?|p_m2]"; eauto.
-    iDestruct "p_m2" as "(%b & % & #? & #?)".
-    iRight. by eauto.
+  - iExists a, gb, kR. by do 3![iSplitR => //].
   - rewrite minted_of_list /= minted_TExp /= minted_TInt minted_TKey.
     rewrite !public_minted !minted_TKey. by do ![iSplitL => //].
   - iIntros "!> _".
     rewrite public_of_list /=.
     by do ![iSplit => //]. }
 wp_pures. wp_apply wp_send => //.
-wp_pures. wp_bind (derive_key _). iApply wp_derive_key.
-pose si := SessInfo kI kR ga gb gab n.
+wp_pures. wp_apply wp_derive_key.
+pose si := SessInfo kI kR ga gb gab.
 iAssert (minted seed) as "#m_seed".
 { rewrite minted_of_list /= !minted_TExp /= minted_TInt.
   by do !iSplit => //; iApply public_minted. }
-iAssert (□ (◇ public seed ↔ ▷ session_fail si))%I as "#s_sec".
-{ iSplitL; last first.
-  { iIntros "!> #comp".
-    rewrite public_of_list /=. do !iSplit => //.
-    iModIntro. iApply public_TExp => //.
-    iApply "s_a". eauto. }
-  iDestruct "p_m2" as "[#?|p_m2]".
-  { iIntros "!> _ !>". by iRight. }
-  iDestruct "p_m2" as "(%b & -> & #s_b & #p_m2)".
-  iIntros "!> #>p_sk".
-  rewrite TExp_TExpN in gab seed secret si *.
-  rewrite /secret /seed public_of_list /= public_TExp2_iff; eauto.
-  iDestruct "p_sk" as "(_ & _ & _ & _ & p_sk & _)".
-  iDestruct "p_sk" as "[[_ #p_b'] | [[_ p_a'] | (_ & a_pred' & _)]]".
-  + iPoseProof ("s_b" with "p_b'") as "p_b". by eauto.
-  + iPoseProof ("s_a" with "p_a'") as "p_a". by eauto.
-  + iPoseProof ("a_pred" with "a_pred'") as ">%contra".
-    by rewrite exps_TExpN in contra. }
-wp_pures. iApply ("Hpost" $! (Some secret)). iFrame.
+wp_pures. iApply ("Hpost" $! (Some secret)).
 iExists si. iFrame. do !iSplitR => //.
-- by rewrite minted_derive_key.
-- iIntros "!> !> %kt".
-  iApply (bi.iff_trans _ (◇ public seed)). iSplit => //.
-  by iApply public_key_derive_key.
-iDestruct "p_m2" as "[#fail|p_m2]".
-{ iLeft. by iRight. }
-iDestruct "p_m2" as "(%b & -> & #p_b & #p_m2)".
-iRight. iFrame. iModIntro. by iSplit.
+  by rewrite minted_derive_key.
+iIntros "!> !> %kt".
+rewrite public_derive_key.
+by iApply public_key_derive_key.
 Qed.
 
 End Verif.
