iso_dh/responder.v
@@ -44,72 +44,49 @@ Definition responder : val := λ: "c" "skR",
 Ltac protocol_failure :=
   by intros; wp_pures; iApply ("Hpost" $! None); iFrame.
 
-Lemma wp_responder c kR dq n :
+Lemma wp_responder c kR :
   channel c -∗
   cryptis_ctx -∗
   iso_dh_ctx N -∗
   public (TKey Open kR) -∗
-  {{{ ●Ph{dq} n }}}
+  {{{ True }}}
     responder c kR
   {{{ okS,
       RET (repr okS);
-      ●Ph{dq} n ∗
       if okS is Some (vkI, kS) then ∃ si,
         ⌜vkI = TKey Open (si_init si)⌝ ∗
         ⌜si_resp si = kR⌝ ∗
         ⌜si_key si = kS⌝ ∗
-        ⌜si_time si = n⌝ ∗
         public vkI ∗
         minted kS ∗
-        □ (∀ kt, public (TKey kt kS) ↔ ▷ session_fail si) ∗
-        session si ∗
+        □ (∀ kt, public (TKey kt kS) ↔ ◇ public kS) ∗
+        (public (TKey Seal (si_init si)) ∨ □ (◇ public kS ↔ ▷ False)) ∗
         term_token (si_resp_share si) ⊤
       else True
  }}}.
 Proof.
 set vkR := TKey Open kR.
-iIntros "#chan_c #? (#? & #?) #p_vkR !> %Φ phase_auth Hpost".
+iIntros "#chan_c #? (#? & #?) #p_vkR !> %Φ _ Hpost".
 wp_lam. wp_pures. wp_apply wp_vkey. wp_pures.
-wp_apply wp_recv => //.
-iIntros "%m1 #p_m1". wp_pures.
+wp_apply wp_recv => //. iIntros "%m1 #p_m1". wp_pures.
 wp_list_of_term m1; last by protocol_failure.
 wp_pures. wp_list_match => [ga vkI -> {m1}|]; last by protocol_failure.
 rewrite public_of_list /=.
 iDestruct "p_m1" as "(p_ga & p_vkI & _)".
-iPoseProof (public_minted with "p_ga") as "m_ga".
-iMod (minted_atI with "[] phase_auth m_ga")
-  as "[phase_auth #ma_ga]"; eauto.
-wp_pures. wp_bind (mknonce _).
-iApply (wp_mknonce_freshN ∅
-          (λ _, (∃ kI, ⌜vkI = TKey Open kI⌝ ∗ public_at n (TKey Seal kI)) ∨
-                public_at n (TKey Seal kR))%I
+wp_pures.
+wp_apply (wp_mknonce_freshN ∅
+          (λ _, False%I)
           iso_dh_pred
-          (λ b, {[TExp (TInt 0) b;
-                  Spec.derive_key (Spec.of_list [vkI; vkR; ga; TExp (TInt 0) b; TExp ga b])]}))
+          (λ b, {[TExp (TInt 0) b]}))
        => //.
 - iIntros "%". rewrite elem_of_empty. iIntros "[]".
 - iIntros "%b".
-  rewrite big_sepS_union_pers.
-  rewrite !big_sepS_singleton minted_derive_key minted_of_list /=.
-  rewrite !minted_TExp minted_TInt /= bi.True_and.
-  iSplit; first by iIntros "!>"; iSplit; iIntros "?".
-  iModIntro. iSplit.
-  + iIntros "#?".
-    iSplit; first by iApply public_minted.
-    iSplit; first by iApply public_minted.
-    by do !iSplit => //.
-  + by iIntros "(_ & _ & _ & _ & (_ & ?) & _)".
+  rewrite big_sepS_singleton minted_TExp minted_TInt /= bi.True_and.
+  iModIntro. by iApply bi.equiv_iff.
 iIntros "%b _ _ #m_b #p_b #dh_gb token".
 set gb := TExp (TInt 0) b.
 set gab := TExp ga b.
-set seed := Spec.of_list [_; _; _; _; _].
-set kS := Spec.derive_key seed.
-have neq: gb ≠ kS
-  by move/(f_equal is_exp); rewrite is_exp_TExp Spec.is_exp_tag.
-rewrite big_sepS_union; last set_solver.
-rewrite {neq} !big_sepS_singleton.
-iDestruct "token" as "[token_gb token_kS]".
-iMod (term_meta_set (nroot.@"info") n with "token_kS") as "#info" => //.
+rewrite big_sepS_singleton.
 iAssert (public gb) as "#p_gb".
 { iApply public_TExp_iff; eauto.
   rewrite minted_TInt. iRight. do ![iSplit => //].
@@ -119,99 +96,55 @@ wp_pure _ credit:"H2".
 wp_apply wp_mkkeyshare => //.
 iIntros "_". wp_pures. wp_list. wp_term_of_list.
 wp_apply wp_sign. wp_pures.
-iPoseProof (phase_auth_frag with "phase_auth") as "#phaseR".
-wp_pures. wp_apply wp_send => //.
+wp_apply wp_send => //.
 { iApply public_TSealIS => //.
   - by rewrite public_minted !minted_TKey.
   - iModIntro.
-    iExists ga, b, vkI, n.  by do ![iSplitL => //].
+    iExists ga, b, vkI.  by do ![iSplitL => //].
   - rewrite minted_of_list /= minted_TExp minted_TInt /=.
     rewrite !public_minted !minted_TKey. by do ![iSplitL => //].
   - iIntros "!> _". rewrite public_of_list /=.
     by eauto. }
-wp_pures. wp_bind (recv _). iApply wp_recv => //.
-iIntros "%m3 #p_m3".
-wp_apply wp_verify.
-case: Spec.decP; last by protocol_failure.
+wp_pures. wp_apply wp_recv => //. iIntros "%m3 #p_m3".
+wp_apply wp_verify. case: Spec.decP; last by protocol_failure.
 move=> kI {}m3 e_vkI ->.
-rewrite {}e_vkI {vkI} in seed kS *. set vkI := TKey Open kI.
+rewrite {}e_vkI {vkI}. set vkI := TKey Open kI.
 wp_pures. wp_list_of_term m3; last by protocol_failure.
 wp_list_match => [ga' gb' vkR' -> {m3}|]; last by protocol_failure.
 wp_eq_term e; last by protocol_failure. subst ga'.
 wp_eq_term e; last by protocol_failure. subst gb'.
 wp_eq_term e; last by protocol_failure. subst vkR'.
 wp_pure _ credit:"H3".
-wp_bind (texp _ _). iApply wp_texp.
+wp_apply wp_texp.
 wp_pure _ credit:"H4".
 iPoseProof (public_TSealE with "p_m3 [//]") as "{p_m3} p_m3".
 rewrite public_of_list /=.
 wp_pures. wp_list. wp_term_of_list.
-wp_pures. rewrite -/seed -/kS. pose si := SessInfo kI kR ga gb gab n.
-iAssert ( |={⊤}=> ●Ph{dq} n ∗
-  □ (session_fail si ∨
-  ∃ a,
-    ⌜ga = TExp (TInt 0) a⌝ ∗
-    (public a ↔ ▷ □ session_fail si) ∗
-    (∀ t, dh_pred a t ↔ ▷ □ iso_dh_pred t)))%I
-  with "[phase_auth H3 H4]"
-  as "{p_m3} > [phase_auth #i_m3]".
-{ iDestruct "p_m3" as "[(p_skI & _) | (#i_m3 & _ & _)]".
-  { iMod (public_atI with "[] H3 phase_auth p_skI")
-      as "[phase_auth #comp]"; eauto => //; try by solve_ndisj.
-    iFrame. iLeft. iIntros "!> !>". by iLeft. }
+wp_pures. pose si := SessInfo kI kR ga gb gab.
+wp_apply wp_derive_key. rewrite -[Spec.derive_key _]/(si_key si).
+iAssert (|={⊤}=> public (TKey Seal kI) ∨ □ (◇ public (si_key si) ↔ ▷ False))%I
+  with "[H4]" as "> #i_m3".
+{ iDestruct "p_m3" as "[(p_skI & _) | (#i_m3 & _ & _)]"; first by eauto.
   iMod (lc_fupd_elim_later_pers with "H4 i_m3") as "{i_m3} #i_m3".
-  iDestruct "i_m3" as "(%a & %gb' & %kR' & %n' & %e_m3 &
-                        p_a & pred_a & i_m3)".
-  case/Spec.of_list_inj: e_m3 => -> <- <- {ga gb' kR'}
-    in gb gab seed kS si *.
-  iDestruct "i_m3" as "[i_m3 | i_m3]".
-  { iPoseProof (public_at_public with "i_m3") as "i_m3'".
-    iMod (public_atI with "[] H3 phase_auth i_m3'")
-      as "[phase_auth #comp]"; eauto => //; try by solve_ndisj.
-    iFrame. iIntros "!> !>". iLeft. by iRight. }
-  rewrite TExp_TExpN TExpC2 -(TExp_TExpN _ [a] b) -/gab -/kS.
-  iPoseProof (term_meta_agree with "info i_m3") as "{i_m3} <-".
-  iFrame. iIntros "!> !>".
-  iRight. iExists a. by do ![iSplitL => //]. }
-iAssert (minted kS) as "#m_kS".
-{ rewrite minted_derive_key minted_of_list /=. do !iSplit => //.
-  - by iApply public_minted.
-  - by iApply public_minted.
-  - by iApply public_minted.
-  - iApply minted_TExp; eauto. }
+  iDestruct "i_m3" as "(%a & %gb' & %kR' & %e_m3 & p_a & pred_a)".
+  case/Spec.of_list_inj: e_m3 => -> _ _ {ga gb' kR'} in gb gab si *.
+  rewrite TExp_TExpN TExpC2 in gab si *.
+  iIntros "!>". iRight. iIntros "!>".
+  iApply (bi.iff_trans _ (◇ public gab)).
+  iSplit; last by iApply public_dh_secret.
+  rewrite public_derive_key public_of_list /=.
+  iSplit; first by iIntros "(_ & _ & _ & _ & p_sk & _)".
+  iIntros "#>p_gab !>". by do !iSplit. }
+iAssert (minted (si_key si)) as "#m_kS".
+{ rewrite minted_derive_key !minted_of_list /= !minted_TExp minted_TInt.
+  by do !iSplit => //; iApply public_minted. }
 iAssert (minted kI) as "#m_kI".
 { iApply minted_TKey. by iApply public_minted. }
 wp_pures.
-iAssert (□ (◇ public seed ↔ ▷ session_fail si))%I as "#sec_sk".
-{ iIntros "!>". iSplit; last first.
-  { iIntros "#comp".
-    rewrite public_of_list /=.
-    do !iSplit => //.
-    iModIntro. iApply public_TExp => //.
-    iApply "p_b".
-    iModIntro. iModIntro.
-    iDestruct "comp" as "[fail|fail]"; eauto. }
-  iIntros "#>p_sk".
-  iDestruct "i_m3" as "[compromise|i_m3]" => //.
-  iDestruct "i_m3" as "(%a & -> & p_a & pred_a)".
-  rewrite TExp_TExpN TExpC2 in gab seed kS si *.
-  rewrite public_of_list /=.
-  iDestruct "p_sk" as "(_ & _ & _ & _ & p_sk & _)".
-  rewrite /gab public_TExp2_iff; eauto.
-  iDestruct "p_sk" as "[[_ p_b'] | [ [_ p_a'] | (_ & contra & _)]]".
-  - iPoseProof ("p_b" with "p_b'") as "fail".
-    iModIntro.
-    iDestruct "fail" as "#[(% & %e & fail)|fail]"; eauto.
-    + case: e => <-. by iLeft.
-    + by iRight.
-  - iPoseProof ("p_a" with "p_a'") as "{p_a} p_a". by eauto.
-  - iPoseProof ("pred_a" with "contra") as ">%contra".
-    by rewrite exps_TExpN in contra. }
-wp_apply wp_derive_key. wp_pures.
-iApply ("Hpost" $! (Some (TKey Open kI, kS))).
-iFrame. iModIntro. iExists si. do !iSplit => //.
+iApply ("Hpost" $! (Some (TKey Open kI, si_key si))).
+iModIntro. iExists si. do !iSplit => //.
 iIntros "!> %kt".
-iApply (bi.iff_trans _ (◇ public seed)); iSplit => //.
+rewrite public_derive_key.
 iApply public_key_derive_key => //.
 by rewrite minted_derive_key.
 Qed.
