iso_dh/shared.v
@@ -17,11 +17,10 @@ Record sess_info := SessInfo {
   si_init_share : term;
   si_resp_share : term;
   si_secret : term;
-  si_time : nat;
 }.
 
 Global Instance sess_info_inhabited : Inhabited sess_info :=
-  populate (SessInfo inhabitant inhabitant inhabitant
+  populate (SessInfo inhabitant inhabitant
               inhabitant inhabitant inhabitant).
 
 Section Verif.
@@ -71,51 +70,36 @@ Definition si_key si :=
                    si_resp_share si;
                    si_secret si]).
 
-Definition session_fail si : iProp :=
-  public_at (si_time si) (TKey Seal (si_init si)) ∨
-  public_at (si_time si) (TKey Seal (si_resp si)).
-
-Definition session si : iProp :=
-  ◯Ph (si_time si) ∗
-  term_meta (si_key si) (nroot.@"info") (si_time si).
-
 Lemma session_agree si1 si2 :
   si_key si1 = si_key si2 →
-  session si1 -∗ session si2 -∗ ⌜si1 = si2⌝.
+  si1 = si2.
 Proof.
-case: si1 si2 => [kI1 kR1 ga1 gb1 gab1 n1] [kI2 kR2 ga2 gb2 gab2 n2] /=.
+case: si1 si2 => [kI1 kR1 ga1 gb1 gab1] [kI2 kR2 ga2 gb2 gab2] /=.
 case/Spec.tag_inj => _.
-case/Spec.of_list_inj => <- <- <- <- <-.
-iIntros "[#hon1 #meta1] [#hon2 #meta2] /=".
-by iPoseProof (term_meta_agree with "meta1 meta2") as "->".
+by case/Spec.of_list_inj => <- <- <- <- <-.
 Qed.
 
 Definition msg2_pred kR m2 : iProp :=
-  ∃ ga b vkI n,
+  ∃ ga b vkI,
     let vkR := TKey Open kR in
     let gb := TExp (TInt 0) b in
     let gab := TExp ga b in
     let secret := Spec.of_list [vkI; vkR; ga; gb; gab] in
     let key := Spec.derive_key secret in
     ⌜m2 = Spec.of_list [ga; gb; vkI]⌝ ∗
-    minted_at n ga ∗
-    (public b ↔ ▷ □ ((∃ kI, ⌜vkI = TKey Open kI⌝ ∗ public_at n (TKey Seal kI)) ∨
-                     public_at n (TKey Seal kR))) ∗
-    (∀ t, dh_pred b t ↔ ▷ □ iso_dh_pred t) ∗
-    term_meta key (nroot.@"info") n.
+    (public b ↔ ▷ □ False) ∗
+    (∀ t, dh_pred b t ↔ ▷ □ iso_dh_pred t).
 
 Definition msg3_pred kI m3 : iProp :=
-  ∃ a gb kR n,
+  ∃ a gb kR,
     let vkI := TKey Open kI in
     let vkR := TKey Open kR in
     let ga := TExp (TInt 0) a in
     let gab := TExp gb a in
-    let si := SessInfo kI kR ga gb gab n in
+    let si := SessInfo kI kR ga gb gab in
     ⌜m3 = Spec.of_list [ga; gb; vkR]⌝ ∗
-    (public a ↔ ▷ □ (public_at n (TKey Seal kI) ∨
-                     public_at n (TKey Seal kR))) ∗
-    (∀ t, dh_pred a t ↔ ▷ □ iso_dh_pred t) ∗
-    (public_at n (TKey Seal kR) ∨ term_meta (si_key si) (nroot.@"info") n).
+    (public a ↔ ▷ □ False) ∗
+    (∀ t, dh_pred a t ↔ ▷ □ iso_dh_pred t).
 
 Definition iso_dh_ctx : iProp :=
   seal_pred (N.@"m2") msg2_pred ∗
@@ -132,6 +116,23 @@ iMod (seal_pred_set (N.@"m2") msg2_pred with "token")
 iMod (seal_pred_set (N.@"m3") msg3_pred with "token")
   as "[#? token]"; try solve_ndisj.
 iModIntro. by iSplit.
+Qed.
+
+Lemma public_dh_secret a b :
+  □ (public a ↔ ▷ □ False) -∗
+  □ (∀ t, dh_pred a t ↔ ▷ □ iso_dh_pred t) -∗
+  □ (public b ↔ ▷ □ False) -∗
+  □ (∀ t, dh_pred b t ↔ ▷ □ iso_dh_pred t) -∗
+  ◇ public (TExpN (TInt 0) [a; b]) ↔ ▷ False.
+Proof.
+iIntros "#s_a #pred_a #s_b #pred_b".
+rewrite public_TExp2_iff //; last by eauto.
+iSplit; last by iIntros ">[]".
+iIntros "> [[_ #p_b] | [[_ #p_a] | (_ & contra & _)]]".
+- by iDestruct ("s_b" with "p_b") as ">[]".
+- by iDestruct ("s_a" with "p_a") as ">[]".
+iPoseProof ("pred_a" with "contra") as ">%contra".
+by rewrite /iso_dh_pred exps_TExpN /= in contra.
 Qed.
 
 End Verif.
